experimenting with putting defns in a locale

src/d_find_ins_del/Find.thy
@@ -49,6 +49,93 @@ constants \<Rightarrow>
   F_finished(r0,k,r,kvs,stk) \<Rightarrow> return (r,kvs,stk)
   | _ \<Rightarrow> failwith (STR ''find 1'')))"
 
+
+(* attempt to do the same, but within a locale *)
+
+locale f =
+  fixes cs :: "constants" and
+  k_cmp :: "'k ord" and
+  frame_ops :: "('k,'r,'frame,'left_half,'right_half,'node) frame_ops" and 
+  store_ops :: "('r,('node,'leaf)dnode,'t) store_ops"
+
+
+definition (in f) find_step :: "
+('k,'r,'leaf,'frame) find_state \<Rightarrow> (('k,'r,'leaf,'frame) find_state,'t) MM" where
+"find_step = (
+  let read = store_ops|>read in
+  (% fs. 
+  case fs of 
+  F_finished _ \<Rightarrow> (failwith (STR ''find_step 1''))
+  | F_down(r0,k,r,stk) \<Rightarrow> (
+    read r |>fmap (% f. 
+    case f of 
+    Disk_node n \<Rightarrow> (        
+      let frm = (frame_ops|>split_node_on_key) n k in
+      let r = (frame_ops|>midpoint) frm in
+      F_down(r0,k,r,frm#stk))
+    | Disk_leaf leaf \<Rightarrow> F_finished(r0,k,r,leaf,stk)))))"
+
+definition (in f) find_big_step :: "
+('k,'r,'leaf,'frame) find_state \<Rightarrow> (('k,'r,'leaf,'frame) find_state,'t) MM" where
+"find_big_step = (
+  (% i.
+  iter_m (% i. case i of
+    F_finished _ \<Rightarrow> (return None)
+    | _ \<Rightarrow> (find_step i |> fmap Some))
+    i))"
+
+
+definition (in f) find :: "'r \<Rightarrow> 'k \<Rightarrow> ('r * 'leaf * 'frame list,'t) MM" where
+"find  r k = (
+  let s = make_initial_find_state k r in
+  find_big_step s |> bind (% s.
+  case s of
+  F_finished(r0,k,r,kvs,stk) \<Rightarrow> return (r,kvs,stk)
+  | _ \<Rightarrow> failwith (STR ''find 1'')))"
+
+print_locale! f
+
+thm f.find_def
+
+definition find2 :: "
+('k,'r,'frame,'left_half,'right_half,'node) frame_ops \<Rightarrow> 
+('r,('node,'leaf)dnode,'t) store_ops \<Rightarrow>  
+'r \<Rightarrow> 'k \<Rightarrow> ('r * 'leaf * 'frame list,'t) MM" where
+"find2 x y = f.find x y"
+
+lemma find_def_2[code]: "find2 x y r k = 
+(let s = make_initial_find_state k r
+     in (case s of
+         F_down prod' \<Rightarrow>
+           (case prod' of
+            (r0, k, r, stk) \<Rightarrow>
+              (y |> read) r |>
+              fmap
+               (case_dnode
+                 (\<lambda>n. let frm = (x |> split_node_on_key) n k in F_down (r0, k, (x |> midpoint) frm, frm # stk))
+                 (\<lambda>leaf. F_finished (r0, k, r, leaf, stk)))) |>
+           fmap Some
+         | F_finished x \<Rightarrow> return None) |>
+        bind
+         (case_option (return s)
+           (iter_m
+             (case_find_state
+               (\<lambda>prod.
+                   (case prod of
+                    (r0, k, r, stk) \<Rightarrow>
+                      (y |> read) r |>
+                      fmap
+                       (case_dnode
+                         (\<lambda>n. let frm = (x |> split_node_on_key) n k
+                               in F_down (r0, k, (x |> midpoint) frm, frm # stk))
+                         (\<lambda>leaf. F_finished (r0, k, r, leaf, stk)))) |>
+                   fmap Some)
+               (\<lambda>x. return None)))) |>
+        bind (\<lambda>s. case s of F_down prod' \<Rightarrow> failwith STR ''find 1'' | F_finished (r0, k, ba) \<Rightarrow> return ba))"
+  apply(simp add: find2_def)
+  apply(simp cong: find_state.case_cong add: f.find_def f.find_big_step_def f.find_step_def)
+  done
+
 end
 
 
