src/d_find_ins_del/Export_code.thy
@@ -50,6 +50,7 @@ Find_state.make_initial_find_state
 dest_F_finished
 (* wellformed_find_state *)
 (* Find_state.wf_trans *)
+find2
 
 
 
